get_tree.sh
@@ -1,7 +1,0 @@
-filename="${1%%.*}"
-options=$2
-
-fpc $2 -vp $1
-rm $filename $filename.o
-mv tree.log $filename.tree.log
-
