tex-fpc/shell/step1.sh
@@ -1,2 +1,0 @@
-./tangle mf/mf.web mf.ch inimf.p mf.pool && fpc -Fasysutils,baseunix,unix inimf.p
-./tangle tex/tex.web tex.ch initex.p tex.pool && fpc -Fasysutils,baseunix,unix initex.p
