tex-fpc/shell/step2.sh
@@ -1,4 +1,0 @@
-cd mf
-../inimf ../lib/plain input ../MFT/local dump
-mv plain.base MFbases
-cd ..
