tex-fpc/shell/step3.sh
@@ -1,5 +1,0 @@
-cd mf
-../ch.ch/mkprod mf
-tangle mf.web mf.ch
-fpc -Fasysutils,baseunix,unix mf.p
-cd ..
