tex-fpc/shell/step5.sh
@@ -1,8 +1,0 @@
-cp lib/hypthen.tex TeXinputs/
-cd tex
-mv ../TeXformats .
-mv ../TeXfonts .
-mv ../TeXinputs .
-../initex ../lib/plain \\dump
-mv plain.fmt TeXformats
-cd ..
