tex-fpc/shell/step6.sh
@@ -1,5 +1,0 @@
-cd tex
-../ch.ch/mkprod tex
-tangle tex.web tex.ch
-fpc -Fasysutils,baseunix,unix tex.p
-cd ..
